added lang stuff

ModelTheory.v
@@ -2,31 +2,39 @@ Require Export Coq.Strings.String.
 Require Export List.
 Require Export Coq.Bool.Bool.
 Require Export Coq.Arith.EqNat.
-
 Notation "x :: l" := (cons x l) (at level 60, right associativity).
 Notation "[ ]" := nil.
 Notation "[ x ; .. ; y ]" := (cons x .. (cons y nil) ..).
 
+(******************************************************************************************)
 (* Symbols *)
+(******************************************************************************************)
+
 Inductive var : Type :=
 | Var : nat -> var.
 Inductive func : Type :=
 | Func : nat -> func.
 Inductive const : Type :=
 | Const : nat -> const.
+Inductive rel : Type :=
+| Rel : nat -> rel.
 
-
+(******************************************************************************************)
 (* Terms *)
+(******************************************************************************************)
+
 Inductive term : Type :=
 | VarT   : var -> term
 | ConstT : const -> term
 | FuncT  : func -> (list term) -> term.
 
+(******************************************************************************************)
 (* Formulas *)
-(* FixMe: does this need a type param? *)
+(******************************************************************************************)
+
 Inductive formula : Type := 
 | Equals  : term -> term -> formula
-| Relates : nat -> (list term) -> formula
+| Relates : rel -> (list term) -> formula
 | Not     : formula -> formula
 | Or      : formula -> formula -> formula
 | Forall  : var -> formula -> formula.
@@ -37,7 +45,10 @@ Definition Impl (phi psi : formula) := Or (Not phi) psi.
 Definition Iff (phi psi : formula) := And (Impl phi psi) (Impl psi phi).
 Definition Exists (v : var) (phi : formula) := Not (Forall v (Not phi)).
 
+(******************************************************************************************)
 (* Subformulas *)
+(******************************************************************************************)
+
 Inductive subformula : formula -> formula -> Prop :=
 | SubIden   (psi phi : formula) : psi = phi -> subformula psi phi
 | SubNot    (psi phi : formula) : subformula (Not psi) phi -> subformula psi phi
@@ -117,7 +128,10 @@ Proof.
   assumption.
 Qed.
 
-(* Util functions for var lists *)
+(******************************************************************************************)
+(* Util functions for var/const/func/rel lists *)
+(******************************************************************************************)
+
 Definition eq_var (v1 : var) (v2 : var) := match v1, v2 with
 | Var v1', Var v2' => beq_nat v1' v2'
 end.
@@ -132,7 +146,37 @@ Fixpoint remove_var (l : list var) (v : var) := match l with
 | h::t => if eq_var v h then remove_var t v else h::(remove_var t v)
 end.
 
-(* Returns vars in a term *)
+Definition eq_const (c1 : const) (c2 : const) := match c1, c2 with
+| Const c1', Const c2' => beq_nat c1' c2'
+end.
+
+Fixpoint contains_const (l : list const) (c : const) := match l with
+| [] => false
+| h::t => eq_const c h || contains_const t c
+end.
+
+Definition eq_func (f1 : func) (f2 : func) := match f1, f2 with
+| Func f1', Func f2' => beq_nat f1' f2'
+end.
+
+Fixpoint contains_func (l : list func) (f : func) := match l with
+| [] => false
+| h::t => eq_func f h || contains_func t f
+end.
+
+Definition eq_rel (r1 : rel) (r2 : rel) := match r1, r2 with
+| Rel r1', Rel r2' => beq_nat r1' r2'
+end.
+
+Fixpoint contains_rel (l : list rel) (r : rel) := match l with
+| [] => false
+| h::t => eq_rel r h || contains_rel t r
+end.
+
+(******************************************************************************************)
+(* Free variables *)
+(******************************************************************************************)
+
 Fixpoint term_vars (t : term) := match t with
 | VarT v    => v::[]
 | ConstT c  => []
@@ -145,7 +189,12 @@ Definition tv := term_vars t.
 Theorem thm : contains_var tv (Var 1) = true. Proof. reflexivity. Qed.
 End term_vars_example.
 
-(* Returns free vars *)
+Definition atomic_func (phi : formula) := match phi with
+| Equals _ _ => true
+| Relates _ _ => true
+| _ => false
+end.
+
 Fixpoint free_vars (phi : formula) := match phi with 
 | Equals t1 t2  => (term_vars t1)++(term_vars t2)
 | Relates _ l   => fold_left (fun a x => a++(term_vars x)) l []
@@ -164,6 +213,10 @@ Theorem thm1 : contains_var fv (Var 1) = false. Proof. reflexivity. Qed.
 Theorem thm2 : contains_var fv (Var 2) = true. Proof. reflexivity. Qed.
 End free_vars_example.
 
+(******************************************************************************************)
+(* Substitution *)
+(******************************************************************************************)
+
 Fixpoint subst_term (t_orig : term) (v : var) (t : term) := match t_orig with
 | VarT v    => t
 | ConstT c  => ConstT c
@@ -171,15 +224,19 @@ Fixpoint subst_term (t_orig : term) (v : var) (t : term) := match t_orig with
 end.
 
 Fixpoint subst_helper (phi: formula) (v : var) (t : term) (free : list var) := match phi with
-| Equals t1 t2  => if (contains_var free v) then Equals (subst_term t1 v t) (subst_term t2 v t) else Equals t1 t2
-| Relates r l   => if (contains_var free v) then Relates r (fold_left (fun a x => (subst_term x v t)::a) l nil) else Relates r l
-| Not psi       => Not (subst_helper psi v t free)
-| Or theta psi  => Or (subst_helper theta v t free) (subst_helper psi v t free)
-| Forall v' psi  => Forall v' (subst_helper psi v t (remove_var free v'))
+| Equals t1 t2  =>  if (contains_var free v) then 
+                      Equals (subst_term t1 v t) (subst_term t2 v t) 
+                    else 
+                      Equals t1 t2
+| Relates r l   =>  if (contains_var free v) then 
+                      Relates r (fold_left (fun a x => (subst_term x v t)::a) l nil) 
+                    else 
+                      Relates r l
+| Not psi       =>  Not (subst_helper psi v t free)
+| Or theta psi  =>  Or (subst_helper theta v t free) (subst_helper psi v t free)
+| Forall v' psi => Forall v' (subst_helper psi v t (remove_var free v'))
 end.
 
-(* Performs a substitution of a variable with a term, only free occurrences should be substituted *)
-(* Note: assumes all the variables in t are substitutable in phi *)
 Definition subst (phi: formula) (v : var) (t : term) := subst_helper phi v t (free_vars phi).
 
 Module subst_example.
@@ -187,8 +244,60 @@ Definition v1       := Var 1.
 Definition v1T      := VarT v1.
 Definition v2T      := VarT (Var 2).
 Definition cT       := ConstT (Const 1).
-Definition phi      := Or (Equals v1T v1T) (Forall v1 (Relates 1 [v1T; v2T])).
+Definition phi      := Or (Equals v1T v1T) (Forall v1 (Relates (Rel 1) [v1T; v2T])).
 Definition phi_sub  := subst phi v1 cT.
-Definition expected := Or (Equals cT cT) (Forall v1 (Relates 1 [v1T; v2T])).
+Definition expected := Or (Equals cT cT) (Forall v1 (Relates (Rel 1) [v1T; v2T])).
 Theorem thm1 : phi_sub = expected. Proof. reflexivity. Qed.
 End subst_example.
+
+(******************************************************************************************)
+(* Languages *)
+(******************************************************************************************)
+
+Inductive lang :=
+| Lang : list const -> list rel -> list func -> lang.
+
+Definition lang_const (l : lang) := match l with
+| Lang c r f => c
+end.
+
+Definition lang_rel (l : lang) := match l with
+| Lang c r f => r
+end.
+
+Definition lang_func (l : lang) := match l with
+| Lang c r f => f
+end.
+
+Fixpoint valid_term (language : lang) (t : term) := match t with
+| VarT _    => true
+| ConstT c  => contains_const (lang_const language) c
+| FuncT f l => contains_func (lang_func language) f && 
+              (fold_left (fun a x => (valid_term language x) && a) l true)
+end.
+
+Fixpoint valid_formula (language : lang) (phi : formula) := match phi with
+| Equals t1 t2  => (valid_term language t1) && (valid_term language t2)
+| Relates r l   => contains_rel (lang_rel language) r &&
+                   (fold_left (fun a x => (valid_term language x) && a) l true)
+| Not psi       => valid_formula language psi
+| Or psi theta  => (valid_formula language psi) && (valid_formula language theta)
+| Forall _ psi  => valid_formula language psi
+end.
+
+Module valid_formula_example.
+Definition c1 := ConstT (Const 1).
+Definition c2 := ConstT (Const 2).
+Definition c3 := ConstT (Const 3).
+Definition v1 := Var 1.
+Definition r1 := (Rel 1).
+Definition phi := Or (Equals c1 c2) (Forall v1 (Relates r1 [VarT v1; c3])).
+Definition l := Lang [Const 1; Const 2; Const 3]  [Rel 1] [].
+Theorem thm1 : (valid_formula l phi) = true. Proof. reflexivity. Qed.
+Definition l' := Lang [Const 1; Const 2] [Rel 1] [].
+Theorem thm2: (valid_formula l' phi) = false. Proof. reflexivity. Qed.
+End valid_formula_example.
+
+(******************************************************************************************)
+(* Models *)
+(******************************************************************************************)
